type/global_tree_ctx.v
@@ -1,0 +1,924 @@
+From mathcomp Require Import ssreflect.seq all_ssreflect.
+From Paco Require Import paco pacotac.
+From SST Require Export src.expressions src.header type.global type.local type.isomorphism type.decidability.
+Require Import List String Coq.Arith.PeanoNat Relations Coq.Logic.Decidable.
+Import ListNotations. 
+(* global trees with context holes *)
+Inductive gtth: Type :=
+  | gtth_hol    : fin -> gtth
+  | gtth_send   : part -> part -> list (option (sort * gtth)) -> gtth.
+
+Section gtth_ind_ref.
+  Variable P : gtth -> Prop.
+  Hypothesis P_hol : forall n, P (gtth_hol n).
+  Hypothesis P_send : forall p q xs, List.Forall (fun u => u = None \/ (exists s g, u = Some(s, g) /\ P g)) xs -> P (gtth_send p q xs).
+  
+  Fixpoint gtth_ind_ref p : P p.
+  Proof.
+    destruct p.
+    - apply P_hol.
+    - apply P_send.
+      induction l; intros; try easy.
+      constructor; try easy.
+      destruct a. 
+      - destruct p. right. exists s1. exists g. split. easy. apply gtth_ind_ref.
+      - left. easy.
+  Qed.
+
+End gtth_ind_ref.
+
+Inductive typ_gtth : list (option gtt) -> gtth -> gtt -> Prop := 
+  | gt_hol : forall n ctx gc, onth n ctx = Some gc -> typ_gtth ctx (gtth_hol n) gc
+  | gt_send : forall ctx p q xs ys, SList xs -> List.Forall2 (fun u v => (u = None /\ v = None) \/ 
+                                                (exists s g g', u = Some(s, g) /\ v = Some(s, g') /\ typ_gtth ctx g g')) xs ys -> 
+                                                typ_gtth ctx (gtth_send p q xs) (gtt_send p q ys).
+
+Section typ_gtth_ind_ref.
+  Variable P : list (option gtt) -> gtth -> gtt -> Prop.
+  Hypothesis P_hol : forall n ctx gc, onth n ctx = Some gc -> P ctx (gtth_hol n ) gc.
+  Hypothesis P_send : forall ctx p q xs ys, SList xs -> List.Forall2 (fun u v => (u = None /\ v = None) \/ 
+                                                 (exists s g g', u = Some(s, g) /\ v = Some(s, g') /\ P ctx g g')) xs ys -> 
+                                                 P ctx (gtth_send p q xs) (gtt_send p q ys).
+  
+  Fixpoint typ_gtth_ind_ref ctx G G' (a : typ_gtth ctx G G') {struct a} : P ctx G G'.
+  Proof.
+    refine (match a with 
+      | gt_hol n ctx gc Ha => P_hol n ctx gc Ha
+      | gt_send ctx p q xs ys Ha Hl => P_send ctx p q xs ys Ha _
+    end); try easy.
+    revert Hl. apply Forall2_mono.
+    intros. 
+    destruct H.
+    - left. easy.
+    - destruct H. destruct H. destruct H. destruct H. destruct H0. subst.
+      right. exists x0. exists x1. exists x2. split. easy. split. easy. 
+      apply typ_gtth_ind_ref; try easy.
+  Qed.
+
+End typ_gtth_ind_ref.
+
+Inductive ishParts : part -> gtth -> Prop := 
+  | ha_sendp : forall p q l, ishParts p (gtth_send p q l)
+  | ha_sendq : forall p q l, ishParts q (gtth_send p q l)
+  | ha_sendr : forall p q r n s g lis, p <> r -> q <> r -> onth n lis = Some (s, g) -> ishParts r g -> ishParts r (gtth_send p q lis).
+
+Lemma ishParts_x : forall [p s1 s2 o1 o2 xs0],
+    (ishParts p (gtth_send s1 s2 (Some (o1,o2) :: xs0)) -> False) ->
+    (ishParts p o2 -> False).
+Proof.
+  intros. apply H. 
+  - case_eq (eqb p s1); intros.
+    assert (p = s1). apply eqb_eq; try easy. subst. apply ha_sendp.
+  - case_eq (eqb p s2); intros.
+    assert (p = s2). apply eqb_eq; try easy. subst. apply ha_sendq.
+  - assert (p <> s1). apply eqb_neq; try easy. 
+    assert (p <> s2). apply eqb_neq; try easy.
+    apply ha_sendr with (n := 0) (s := o1) (g := o2); try easy.
+Qed.
+
+
+Lemma ishParts_hxs : forall [p s1 s2 o1 xs0],
+    (ishParts p (gtth_send s1 s2 (o1 :: xs0)) -> False) ->
+    (ishParts p (gtth_send s1 s2 xs0) -> False).
+Proof.
+  intros. apply H.
+  inversion H0. subst. apply ha_sendp. apply ha_sendq.
+  subst. apply ha_sendr with (n := Nat.succ n) (s := s) (g := g); try easy.
+Qed.
+
+Lemma ishParts_n : forall [n p s s' xs s0 g],
+    (ishParts p (gtth_send s s' xs) -> False) ->
+    onth n xs = Some(s0, g) -> 
+    (ishParts p g -> False).
+Proof.  
+  induction n; intros; try easy.
+  - apply H. destruct xs; try easy. simpl in *. subst.
+    - case_eq (eqb p s); intros.
+      assert (p = s). apply eqb_eq; try easy. subst. apply ha_sendp.
+    - case_eq (eqb p s'); intros.
+      assert (p = s'). apply eqb_eq; try easy. subst. apply ha_sendq.
+    - assert (p <> s). apply eqb_neq; try easy. 
+      assert (p <> s'). apply eqb_neq; try easy.
+      apply ha_sendr with (n := 0) (s := s0) (g := g); try easy.
+  - destruct xs; try easy.
+    specialize(ishParts_hxs H); intros.
+    specialize(IHn p s s' xs s0 g). apply IHn; try easy.
+Qed.
+
+Lemma Forall3S_to_Forall2_r : forall ctxG0 ctxG1 ctxG,
+    Forall3S
+       (fun u v w : option gtt =>
+        u = None /\ v = None /\ w = None \/
+        (exists t : gtt, u = None /\ v = Some t /\ w = Some t) \/
+        (exists t : gtt, u = Some t /\ v = None /\ w = Some t) \/
+        (exists t : gtt, u = Some t /\ v = Some t /\ w = Some t)) ctxG0 ctxG1 ctxG -> 
+    Forall2R 
+        (fun u v => (u = None \/ u = v)) ctxG1 ctxG.
+Proof.
+  induction ctxG0; intros.
+  inversion H. subst.
+  - clear H. induction ctxG; intros; try easy. constructor; try easy. right. right. easy. easy.
+  - subst. constructor.
+  - inversion H.
+    - subst. specialize(IHctxG0 nil ctxG0). constructor.
+    - subst. clear H.
+      specialize(IHctxG0 xb xc H6). constructor; try easy.
+      clear H6 IHctxG0.
+      destruct H3. destruct H as (Ha,(Hb,Hc)). subst. left. easy.
+      destruct H. destruct H as (t,(Ha,(Hb,Hc))). subst. right. easy.
+      destruct H. destruct H as (t,(Ha,(Hb,Hc))). subst. left. easy.
+      destruct H as (t,(Ha,(Hb,Hc))). subst. right. easy.
+Qed.
+
+Lemma Forall3S_to_Forall2_l : forall ctxG0 ctxG1 ctxG,
+    Forall3S
+       (fun u v w : option gtt =>
+        u = None /\ v = None /\ w = None \/
+        (exists t : gtt, u = None /\ v = Some t /\ w = Some t) \/
+        (exists t : gtt, u = Some t /\ v = None /\ w = Some t) \/
+        (exists t : gtt, u = Some t /\ v = Some t /\ w = Some t)) ctxG0 ctxG1 ctxG -> 
+    Forall2R 
+        (fun u v => (u = None \/ u = v)) ctxG0 ctxG.
+Proof.
+  induction ctxG0; intros.
+  inversion H. subst. constructor. constructor.
+  - inversion H.
+    - subst. constructor. right. easy. specialize(IHctxG0 nil ctxG0). apply IHctxG0. constructor.
+    - subst. clear H.
+      specialize(IHctxG0 xb xc H6). constructor; try easy.
+      clear H6 IHctxG0.
+      destruct H3. destruct H as (Ha,(Hb,Hc)). subst. left. easy.
+      destruct H. destruct H as (t,(Ha,(Hb,Hc))). subst. left. easy.
+      destruct H. destruct H as (t,(Ha,(Hb,Hc))). subst. right. easy.
+      destruct H as (t,(Ha,(Hb,Hc))). subst. right. easy.
+Qed.
+
+Inductive isMergeCtx : list (option gtt) -> list (option (list (option gtt))) -> Prop :=   
+  | cmatm : forall t, isMergeCtx t (Some t :: nil)
+  | cmconsn : forall t xs, isMergeCtx t xs -> isMergeCtx t (None :: xs) 
+  | cmconss : forall t t' t'' xs, 
+      Forall3S (fun u v w => 
+        (u = None /\ v = None /\ w = None) \/
+        (exists t, u = None /\ v = Some t /\ w = Some t) \/
+        (exists t, u = Some t /\ v = None /\ w = Some t) \/
+        (exists t, u = Some t /\ v = Some t /\ w = Some t)
+      ) t t' t'' ->
+      isMergeCtx t xs -> isMergeCtx t'' (Some t' :: xs). 
+
+
+
+Inductive usedCtx : (list (option gtt)) -> gtth -> Prop := 
+  | used_hol : forall n G, usedCtx (extendLis n (Some G)) (gtth_hol n)
+  | used_con : forall ctxG ctxGLis p q ys, isMergeCtx ctxG ctxGLis -> 
+        List.Forall2 (fun u v => (u = None /\ v = None) \/ (exists ctxGi s g, u = Some ctxGi /\ v = Some (s, g) /\ usedCtx ctxGi g)) ctxGLis ys -> usedCtx ctxG (gtth_send p q ys).
+
+Lemma mergeCtx_to_2R : forall ctxGLis ctxG,
+    isMergeCtx ctxG ctxGLis -> 
+    Forall (fun u => u = None \/ (exists ctxGi, u = Some ctxGi /\
+      Forall2R (fun u v => (u = None \/ u = v)) ctxGi ctxG
+    )) ctxGLis.
+Proof.
+  induction ctxGLis; intros; try easy.
+  inversion H.
+  - subst. constructor; try easy. right. exists ctxG.
+    split. easy. clear H IHctxGLis. induction ctxG; intros.
+    constructor. constructor; try easy. right. easy.
+  - subst. specialize(IHctxGLis ctxG H2). constructor; try easy. left. easy.
+  - subst.
+    specialize(IHctxGLis t H4). clear H.
+    constructor.
+    - right. exists t'. split. easy.
+      clear H4 IHctxGLis.
+      apply Forall3S_to_Forall2_r with (ctxG0 := t); try easy.
+      revert IHctxGLis. apply Forall_mono; intros.
+      destruct H. left. easy.
+      destruct H as (ctxGi,(Ha,Hb)). subst. right. exists ctxGi. split. easy.
+      specialize(Forall3S_to_Forall2_l t t' ctxG H3); intros.
+      clear H3 H4. clear ctxGLis t'.
+      revert Hb H. revert t ctxG.
+      induction ctxGi; intros; try easy.
+      - constructor.
+      - destruct t; try easy. destruct ctxG; try easy.
+        inversion Hb. subst. clear Hb. inversion H. subst. clear H.
+        specialize(IHctxGi t ctxG H5 H7). constructor; try easy.
+        clear H5 H7.
+        destruct H3. left. easy.
+        subst. destruct H4. left. easy. subst. right. easy.
+Qed.
+
+Lemma typh_with_more : forall gl ctxJ ctxG g3,
+            typ_gtth ctxJ gl g3 -> 
+            Forall2R (fun u v : option gtt => u = None \/ u = v) ctxJ ctxG -> 
+            typ_gtth ctxG gl g3.
+Proof.
+  induction gl using gtth_ind_ref; intros.
+  - inversion H. subst. constructor.
+    clear H. revert H3 H0. revert ctxG ctxJ. induction n; intros.
+    - destruct ctxJ; try easy. destruct ctxG; try easy.
+      inversion H0. subst. clear H0.
+      simpl in H3. subst. destruct H4; try easy. 
+    - destruct ctxJ; try easy. destruct ctxG; try easy.
+      inversion H0. subst. clear H0.
+      specialize(IHn ctxG ctxJ). apply IHn; try easy.
+  - inversion H0. subst. constructor; try easy.
+    clear H7 H0. revert H8 H1 H.
+    revert xs ctxJ ctxG. clear p q.
+    induction ys; intros.
+    - destruct xs; try easy.
+    - destruct xs; try easy. inversion H. subst. clear H. inversion H8. subst. clear H8.
+      specialize(IHys xs ctxJ ctxG H7 H1 H4). constructor; try easy. clear H7 H4 IHys.
+      destruct H5. left. easy.
+      destruct H as (s1,(g1,(g2,(Ha,(Hb,Hc))))). subst.
+      destruct H3; try easy. destruct H as (s2,(g3,(Hd,He))). inversion Hd. subst.
+      right. exists s2. exists g3. exists g2. split. easy. split. easy.
+      specialize(He ctxJ ctxG g2). apply He; try easy.
+Qed.
+
+Lemma typ_gtth_pad_l : forall Gl' g1 ctxJ ctxG,
+    typ_gtth (noneLis (Datatypes.length ctxJ) ++ ctxG) Gl' g1 -> 
+    typ_gtth (ctxJ ++ ctxG)%list Gl' g1.
+Proof.
+  intros.
+  specialize(typh_with_more Gl' (noneLis (Datatypes.length ctxJ) ++ ctxG) (ctxJ ++ ctxG) g1); intros. apply H0; try easy.
+  clear H0 H. induction ctxJ; intros; try easy.
+  - simpl. induction ctxG; intros; try easy. constructor. constructor; try easy. right. easy.
+  - constructor; try easy. left. easy.
+Qed.
+
+Lemma typ_gtth_pad_r : forall g2 g3 ctxJ ctxG,
+        typ_gtth ctxJ g2 g3 -> 
+        typ_gtth (ctxJ ++ ctxG)%list g2 g3.
+Proof.
+  intros.
+  specialize(typh_with_more g2 ctxJ (ctxJ ++ ctxG) g3); intros.
+  apply H0; try easy.
+  clear H0 H. induction ctxJ; intros; try easy. constructor.
+  constructor; try easy. right. easy.
+Qed.
+
+Lemma typh_with_less : forall ctxGi' ctxG g4 g3,
+            typ_gtth ctxG g4 g3 -> 
+            Forall2R (fun u v : option gtt => u = None \/ u = v) ctxGi' ctxG -> 
+            usedCtx ctxGi' g4 -> 
+            typ_gtth ctxGi' g4 g3.
+Proof.
+  intros. revert H H0 H1. revert g3 ctxGi' ctxG.
+  induction g4 using gtth_ind_ref; intros.
+  - inversion H. subst. constructor; try easy. 
+    inversion H1. subst.
+    clear H1 H. revert H4 H0. revert g3 ctxG G. induction n; intros; try easy.
+    - destruct ctxG; try easy. simpl in H4. subst.
+      inversion H0. subst. simpl. destruct H3; try easy.
+    - destruct ctxG; try easy. inversion H0. subst. 
+      apply IHn with (ctxG := ctxG); try easy.
+  - inversion H0. subst.
+    constructor; try easy. 
+    inversion H2. subst.
+    specialize(mergeCtx_to_2R ctxGLis ctxGi' H6); intros. clear H6 H8 H2 H0.
+    revert H3 H10 H9 H1 H. revert ctxGi' ctxG ys ctxGLis. clear p q.
+    induction xs; intros; try easy.
+    - destruct ys; try easy.
+    - destruct ys; try easy. destruct ctxGLis; try easy.
+      inversion H. subst. clear H. inversion H9. subst. clear H9.
+      inversion H3. subst. clear H3. inversion H10. subst. clear H10.
+      specialize(IHxs ctxGi' ctxG ys ctxGLis).
+      assert(Forall2
+         (fun (u : option (sort * gtth)) (v : option (sort * gtt)) =>
+          u = None /\ v = None \/
+          (exists (s : sort) (g : gtth) (g' : gtt),
+             u = Some (s, g) /\ v = Some (s, g') /\ typ_gtth ctxGi' g g')) xs ys).
+      apply IHxs; try easy. constructor; try easy.
+      clear H H12 H7 H8 H5 IHxs.
+      destruct H6. left. easy.
+      destruct H as (s1,(g1,(g2,(Ha,(Hb,Hc))))). subst.
+      destruct H4; try easy. destruct H as (s2,(g3,(Hd,He))). inversion Hd. subst.
+      destruct H9; try easy. destruct H as (ct,(s3,(g4,(Hf,(Hg,Hh))))). inversion Hg. subst.
+      destruct H2; try easy. destruct H as (ct2,(Hi,Hj)). inversion Hi. subst.
+      right. exists s3. exists g4. exists g2.
+      split. easy. split. easy.
+      specialize(He g2 ct2 ctxG).
+      assert(typ_gtth ct2 g4 g2).
+      {
+        apply He; try easy.
+        clear Hh Hi Hc Hd He Hg. 
+        revert Hj H1. revert ctxGi' ctxG.
+        induction ct2; intros; try easy.
+        - constructor.
+        - destruct ctxGi'; try easy. destruct ctxG; try easy.
+          inversion Hj. subst. clear Hj. inversion H1. subst. clear H1.
+          specialize(IHct2 ctxGi' ctxG H5 H7). constructor; try easy.
+          destruct H3. left. easy. subst. destruct H4. left. easy. subst. right. easy.
+      }
+      apply typh_with_more with (ctxJ := ct2); try easy.
+Qed.
+
+Lemma typh_with_more2 {A} : forall ctxGi' ctxG (ctxJ : list A) gl g3,
+            typ_gtth (noneLis (Datatypes.length ctxJ) ++ ctxGi') gl g3 -> 
+            Forall2R (fun u v : option gtt => u = None \/ u = v) ctxGi' ctxG -> 
+            typ_gtth (noneLis (Datatypes.length ctxJ) ++ ctxG) gl g3.
+Proof.
+  intros.
+  apply typh_with_more with (ctxJ := (noneLis (Datatypes.length ctxJ) ++ ctxGi')); try easy.
+  clear H.
+  induction ctxJ; intros; try easy.
+  constructor; try easy. left. easy.
+Qed.
+
+Lemma ctx_back : forall s s' xs ys0 ctxG,
+      typ_gtth ctxG (gtth_send s s' xs) (gtt_send s s' ys0) -> 
+      usedCtx ctxG (gtth_send s s' xs) -> 
+      exists ctxGLis, 
+      Forall3 (fun u v w => (u = None /\ v = None /\ w = None) \/ (exists ct s g g', u = Some ct /\ v = Some(s, g) /\ w = Some(s, g') /\ typ_gtth ct g g' /\ usedCtx ct g)) ctxGLis xs ys0 /\
+      isMergeCtx ctxG ctxGLis.
+Proof.
+  intros.
+  inversion H. subst. clear H.
+  inversion H0. subst. clear H0.
+  clear H4. clear s s'.
+  specialize(mergeCtx_to_2R ctxGLis ctxG H3); intros. 
+  exists ctxGLis. split; try easy. clear H3.
+  revert H7 H6 H. revert ys0 ctxG ctxGLis.
+  induction xs; intros.
+  - destruct ys0; try easy. destruct ctxGLis; try easy. constructor.
+  - destruct ys0; try easy. destruct ctxGLis; try easy.
+    inversion H7. subst. clear H7. inversion H6. subst. clear H6.
+    inversion H. subst. clear H.
+    specialize(IHxs ys0 ctxG ctxGLis H5 H8 H6). constructor; try easy.
+    clear H6 H8 H5 IHxs.
+    - destruct H4. destruct H. subst. destruct H3. destruct H. subst. left. easy.
+      destruct H as (s1,(g1,(g2,Ha))). easy.
+    - destruct H as (ct,(s1,(g1,(Ha,(Hb,Hc))))). subst.
+      destruct H3; try easy. destruct H as (s2,(g2,(g3,(Hd,(He,Hf))))). inversion Hd. subst.
+      destruct H2; try easy. destruct H as (ct2,(Hg,Hh)). inversion Hg. subst.
+      right. exists ct2. exists s2. exists g2. exists g3.
+      split. easy. split. easy. split. easy. split; try easy.
+      apply typh_with_less with (ctxG := ctxG); try easy.
+Qed.
+
+Lemma mergeCtx_sl : forall n ctxGLis ctxGi ctxG,
+        onth n ctxGLis = Some ctxGi -> 
+        isMergeCtx ctxG ctxGLis -> 
+        Forall2R (fun u v => u = v \/ u = None) ctxGi ctxG.
+Proof.
+  induction n; intros.
+  - destruct ctxGLis; try easy. 
+    simpl in H. subst.
+    inversion H0. subst. 
+    - clear H0. induction ctxGi; intros; try easy. constructor.
+      constructor; try easy. left. easy.
+    - subst.
+      clear H4 H0. clear ctxGLis.
+      revert H3. revert ctxG t. induction ctxGi; intros; try easy.
+      - constructor.
+      - inversion H3; try easy.
+        - subst. clear H3 IHctxGi. constructor. left. easy. clear a.
+          induction ctxGi; intros; try easy. constructor. constructor; try easy. left. easy.
+        - subst. specialize(IHctxGi xc xa H6). constructor; try easy.
+          clear H3 H6. 
+          - destruct H4. destruct H as (Ha,(Hb,Hc)). subst. left. easy.
+          - destruct H. destruct H as (t1,(Ha,(Hb,Hc))). subst. left. easy.
+          - destruct H. destruct H as (t1,(Ha,(Hb,Hc))). subst. right. easy.
+          - destruct H as (t1,(Ha,(Hb,Hc))). subst. left. easy.
+  - destruct ctxGLis; try easy.
+    inversion H0; try easy.
+    - subst. destruct n; try easy.
+    - subst. specialize(IHn ctxGLis ctxGi ctxG). apply IHn; try easy.
+    - subst. specialize(IHn ctxGLis ctxGi t H H5).
+      clear H0 H H5.
+      clear ctxGLis n.
+      revert H4 IHn. revert t ctxG t'.
+      induction ctxGi; intros; try easy.
+      - constructor.
+      - inversion H4. 
+        - subst. inversion IHn; try easy.
+        - subst. destruct ctxG; try easy.
+        - subst. clear H4.
+          inversion IHn. subst. clear IHn.
+          specialize(IHctxGi xa xc xb H0 H6). constructor; try easy.
+          clear IHctxGi H0 H6.
+          destruct H4. subst.
+          - destruct H. destruct H as (Ha,(Hb,Hc)). subst. left. easy.
+          - destruct H. destruct H as (t1,(Ha,(Hb,Hc))). subst. right. easy.
+          - destruct H. destruct H as (t1,(Ha,(Hb,Hc))). subst. left. easy.
+          - destruct H as (t1,(Ha,(Hb,Hc))). subst. left. easy.
+          subst. right. easy.
+Qed.
+
+
+Lemma shift_to : forall (g1 : gtt) (p : string) (Gl : gtth) (ctxG ctxJ : seq.seq (option gtt)),
+typ_gtth ctxG Gl g1 ->
+(ishParts p Gl -> False) ->
+usedCtx ctxG Gl ->
+exists Gl' : gtth,
+  typ_gtth (noneLis (Datatypes.length ctxJ) ++ ctxG) Gl' g1 /\
+  usedCtx (noneLis (Datatypes.length ctxJ) ++ ctxG) Gl' /\ (ishParts p Gl' -> False).
+Proof.
+  intros g1 p Gl. revert g1 p.
+  induction Gl using gtth_ind_ref; intros; try easy.
+  - inversion H1. subst.
+    exists (gtth_hol ((Datatypes.length ctxJ) + n)).
+    assert(extendLis (Datatypes.length ctxJ + n) (Some G) =
+     (noneLis (Datatypes.length ctxJ) ++ extendLis n (Some G))%SEQ).
+      {
+       clear H1 H0 H. clear g1 p. induction ctxJ; intros; try easy.
+       simpl in *. replace (extendLis (Datatypes.length ctxJ + n)%Nrec (Some G))%SEQ with
+          ((noneLis (Datatypes.length ctxJ) ++ extendLis n (Some G))%SEQ). easy. 
+      }
+      rename H2 into Ht.
+    split.
+    - inversion H. subst. 
+      specialize(extendExtract n (Some G)); intros.
+      specialize(eq_trans (esym H4) H2); intros. inversion H3. subst.
+      clear H4 H3 H2.
+      constructor. clear H1 H0 H Ht. clear p. revert G n.
+      induction ctxJ; intros; try easy. simpl in *.
+      apply extendExtract; try easy.
+      specialize(IHctxJ G n). easy.
+    - split.
+      replace ((noneLis (Datatypes.length ctxJ) ++ extendLis n (Some G))%SEQ) with (extendLis (Datatypes.length ctxJ + n) (Some G)). constructor.
+    - intros. inversion H2; try easy.
+  - inversion H0. subst.
+    inversion H2. subst.
+    assert(
+      exists zs,
+      Forall2 (fun u v => (u = None /\ v = None) \/ exists s g g', u = Some(s, g) /\ v = Some(s, g') /\ typ_gtth (noneLis (Datatypes.length ctxJ) ++ ctxG) g g') zs ys /\
+      List.Forall2 (fun u v => (u = None /\ v = None) \/ (exists ctxGi s g, u = Some ctxGi /\ v = Some (s, g) /\ usedCtx (noneLis (Datatypes.length ctxJ) ++ ctxGi) g)) ctxGLis zs /\
+      Forall (fun u => u = None \/ (exists s g, u = Some(s, g) /\ (ishParts p0 g -> False))) zs 
+    ). 
+    {
+      specialize(mergeCtx_to_2R ctxGLis ctxG H6); intros.
+      clear H6 H8 H2 H0.
+      revert H H1 H9 H10 H3.
+      revert p q xs p0 ctxG ctxJ ctxGLis.
+      induction ys; intros; try easy.
+      - destruct xs; try easy. destruct ctxGLis; try easy.
+        exists nil. easy.
+      - destruct xs; try easy. destruct ctxGLis; try easy.
+        inversion H9. subst. clear H9. inversion H10. subst. clear H10.
+        inversion H3. subst. clear H3. inversion H. subst. clear H.
+        assert(exists zs : seq.seq (option (sort * gtth)),
+         Forall2
+           (fun (u : option (sort * gtth)) (v : option (sort * gtt)) =>
+            u = None /\ v = None \/
+            (exists (s : sort) (g : gtth) (g' : gtt),
+               u = Some (s, g) /\
+               v = Some (s, g') /\ typ_gtth (noneLis (Datatypes.length ctxJ) ++ ctxG) g g')) zs ys /\
+         Forall2
+           (fun (u : option (seq.seq (option gtt))) (v : option (sort * gtth)) =>
+            u = None /\ v = None \/
+            (exists (ctxGi : seq.seq (option gtt)) (s : sort) (g : gtth),
+               u = Some ctxGi /\
+               v = Some (s, g) /\ usedCtx (noneLis (Datatypes.length ctxJ) ++ ctxGi) g)) ctxGLis zs /\
+         Forall
+           (fun u : option (sort * gtth) =>
+            u = None \/ (exists (s : sort) (g : gtth), u = Some (s, g) /\ (ishParts p0 g -> False))) zs).
+        specialize(IHys p q xs p0 ctxG ctxJ ctxGLis). apply IHys; try easy.
+        specialize(ishParts_hxs H1); try easy.
+        clear IHys H10 H8 H9 H7.
+        destruct H as (zs,(Ha,(Hb,Hc))).
+        destruct H6.
+        - destruct H. subst. destruct H5. destruct H. subst.
+          exists (None :: zs).
+          - split. constructor; try easy. left. easy.
+          - split. constructor; try easy. left. easy.
+          - constructor; try easy. left. easy.
+          destruct H as (s1,(g1,(g2,Ht))). easy.
+        - destruct H as (ctxGi,(s1,(g1,(Hd,(He,Hf))))). subst.
+          destruct H5; try easy. destruct H as (s2,(g2,(g3,(Hg,(Hh,Hi))))). inversion Hg. subst.
+          destruct H4; try easy. destruct H as (ctxGi',(Hj,Hk)). inversion Hj. subst.
+          destruct H3; try easy. destruct H as (s3,(g4,(Hl,Hm))). inversion Hl. subst.
+          specialize(Hm g3 p0 ctxGi' ctxJ).
+          assert(exists Gl' : gtth,
+       typ_gtth (noneLis (Datatypes.length ctxJ) ++ ctxGi') Gl' g3 /\
+       usedCtx (noneLis (Datatypes.length ctxJ) ++ ctxGi') Gl' /\ (ishParts p0 Gl' -> False)).
+          {
+            apply Hm; try easy.
+            - apply typh_with_less with (ctxG := ctxG); try easy.
+            - specialize(ishParts_x H1); try easy.
+          }
+          destruct H as (gl,(Hd,(He,Hta))). exists (Some (s3, gl) :: zs).
+          - split. constructor; try easy.
+            right. exists s3. exists gl. exists g3. split. easy. split. easy.
+            apply typh_with_more2 with (ctxGi' := ctxGi'); try easy.
+          - split. constructor; try easy. right. exists ctxGi'. exists s3. exists gl. easy.
+          - constructor; try easy. right. exists s3. exists gl. easy.
+    } 
+    destruct H3 as (zs,(Ha,(Hb,Hc))).
+    exists (gtth_send p q zs).
+    - split. constructor; try easy.
+      clear H H0 H1 H2 H6 H10 Hb Hc. 
+      revert Ha H9 H8. revert ctxG ctxJ ys zs. clear p q p0 ctxGLis.
+      induction xs; intros; try easy.
+      specialize(SList_f a xs H8); intros.
+      destruct ys; try easy. destruct zs; try easy. inversion Ha. subst. clear Ha. 
+      inversion H9. subst. clear H9.
+      destruct H.
+      - specialize(IHxs ctxG ctxJ ys zs). apply SList_b. apply IHxs; try easy.
+      - destruct H as (H,(a0,Ha)). subst. 
+        destruct ys; try easy. destruct zs; try easy. clear H7 H5 H8 IHxs.
+        destruct H4; try easy.
+        destruct H as (s1,(g1,(g2,(Ha,(Hb,Hc))))). subst.
+        destruct H3; try easy. destruct H as (s2,(g3,(g4,(Hd,(He,Hf))))). subst. easy.
+    - split.
+      assert(exists ks, Forall2 (fun u v => (u = None /\ v = None) \/ (exists ctxGi ctxGi', u = Some ctxGi /\ v = Some ctxGi' /\ (noneLis (Datatypes.length ctxJ) ++ ctxGi) = ctxGi')) ctxGLis ks).
+      {
+        clear Hc Hb Ha H10 H6 H9 H8 H2 H1 H0 H.
+        induction ctxGLis; intros; try easy.
+        exists nil. easy.
+        destruct IHctxGLis as (ks, H).
+        destruct a.
+        - exists (Some (noneLis (Datatypes.length ctxJ) ++ l) :: ks). constructor; try easy.
+          right. exists l. exists (noneLis (Datatypes.length ctxJ) ++ l). easy.
+        - exists (None :: ks). constructor; try easy. left. easy.
+      }
+      destruct H3 as (ks, H3).
+      clear Hc Ha H10 H9 H8 H2 H1 H0 H.
+      clear p0 ys. 
+      apply used_con with (ctxGLis := ks); try easy.
+      - clear Hb. revert H3 H6. 
+        revert ctxG ctxJ ks. clear p q xs zs.
+        induction ctxGLis; intros; try easy.
+        destruct ks; try easy. inversion H3. subst. clear H3.
+        inversion H6.
+        - subst. destruct ks; try easy. destruct H2; try easy.
+          destruct H as (ct1,(ct2,(Ha,(Hb,Hc)))). inversion Ha. subst. constructor.
+        - subst. destruct H2. destruct H. subst.
+          specialize(IHctxGLis ctxG ctxJ ks). 
+          assert(isMergeCtx (noneLis (Datatypes.length ctxJ) ++ ctxG) ks). apply IHctxGLis; try easy.
+          constructor. easy.
+          destruct H as (ct1,(ct2,Ha)). easy.
+        - subst. specialize(IHctxGLis t ctxJ ks H5 H4).
+          destruct H2; try easy. destruct H as (ct1,(ct2,(Ha,(Hb,Hc)))). inversion Ha. subst.
+          apply cmconss with (t := (noneLis (Datatypes.length ctxJ) ++ t)); try easy.
+          clear H4 H5 Ha H6 IHctxGLis. induction ctxJ; intros; try easy.
+          simpl. constructor; try easy. left. easy.
+      - revert H3 Hb. clear H6.
+        revert ctxJ zs ks. clear p q xs ctxG.
+        induction ctxGLis; intros.
+        - destruct ks; try easy. destruct zs; try easy.
+        - destruct ks; try easy. destruct zs; try easy. 
+          inversion H3. subst. clear H3. inversion Hb. subst. clear Hb.
+          specialize(IHctxGLis ctxJ zs ks H5 H6). constructor; try easy.
+          clear IHctxGLis H5 H6.
+          - destruct H2. destruct H. subst. destruct H3. destruct H. subst. left. easy.
+            destruct H as(ct,(s1,(g1,Ha))). easy.
+          - destruct H as (ct1,(ct2,(Ha,(Hb,Hc)))). subst.
+            destruct H3; try easy. destruct H as (ct2,(s2,(g2,(Ha,(Hb,Hc))))). inversion Ha. subst.
+            right. exists (noneLis (Datatypes.length ctxJ) ++ ct2). exists s2. exists g2. easy.
+    - intros.
+      inversion H3. 
+      - subst. apply H1. constructor.
+      - subst. apply H1. constructor.
+      - subst. specialize(some_onth_implies_In n zs (s, g) H14); intros.
+        specialize(Forall_forall (fun u : option (sort * gtth) =>
+        u = None \/ (exists (s : sort) (g : gtth), u = Some (s, g) /\ (ishParts p0 g -> False))) zs); intros.
+        destruct H5. specialize(H5 Hc). clear H7 Hc.
+        specialize(H5 (Some(s, g)) H4). destruct H5; try easy.
+        destruct H5 as (s1,(g1,(Hta,Htb))). inversion Hta. subst.
+        apply Htb; try easy.
+Qed.
+
+Lemma ctx_merge : forall s s0 s1 g1 l p,
+    p <> s -> p <> s0 ->
+    (exists (G' : gtth) (ctxG : seq.seq (option gtt)),
+       typ_gtth ctxG G' g1 /\
+       (ishParts p G' -> False) /\
+       Forall
+         (fun u : option gtt =>
+          u = None \/
+          (exists (q : string) (lsg : seq.seq (option (sort * gtt))),
+             u = Some (gtt_send p q lsg) \/ u = Some (gtt_send q p lsg) \/ u = Some gtt_end)) ctxG /\
+       usedCtx ctxG G') -> 
+       (exists (G' : gtth) (ctxG : seq.seq (option gtt)),
+       typ_gtth ctxG G' (gtt_send s s0 l) /\
+       (ishParts p G' -> False) /\
+       Forall
+         (fun u : option gtt =>
+          u = None \/
+          (exists (q : string) (lsg : seq.seq (option (sort * gtt))),
+             u = Some (gtt_send   p q lsg) \/ u = Some (gtt_send q p lsg) \/ u = Some gtt_end)) ctxG /\
+       usedCtx ctxG G') -> 
+       (exists (G' : gtth) (ctxG : seq.seq (option gtt)),
+  typ_gtth ctxG G' (gtt_send s s0 (Some (s1, g1) :: l)) /\
+  (ishParts p G' -> False) /\
+  Forall
+    (fun u : option gtt =>
+     u = None \/
+     (exists (q : string) (lsg : seq.seq (option (sort * gtt))),
+        u = Some (gtt_send p q lsg) \/ u = Some (gtt_send q p lsg) \/ u = Some gtt_end)) ctxG /\
+  usedCtx ctxG G').
+Proof.
+  intros.
+  destruct H1 as (Gl,(ctxG,(Ha,(Hb,(Hc,Hd))))).
+  destruct H2 as (Gl2,(ctxJ,(He,(Hf,(Hg,Hh))))).
+  inversion He. subst.
+  - specialize(some_onth_implies_In n ctxJ (gtt_send s s0 l) H1); intros.
+    specialize(Forall_forall (fun u : option gtt =>
+        u = None \/
+        (exists (q : string) (lsg : seq.seq (option (sort * gtt))),
+           u = Some (gtt_send p q lsg) \/ u = Some (gtt_send q p lsg) \/ u = Some gtt_end)) ctxJ); intros.
+    destruct H3. specialize(H3 Hg). clear H4 Hg.
+    specialize(H3 (Some (gtt_send s s0 l)) H2). destruct H3; try easy.
+    destruct H3 as (q1,(lsg,H3)).
+    - destruct H3. inversion H3. subst. easy.
+    - destruct H3. inversion H3. subst. easy.
+    - inversion H3.
+  - subst.
+    assert(exists Gl', typ_gtth (noneLis (List.length ctxJ) ++ ctxG) Gl' g1 /\ usedCtx (noneLis (List.length ctxJ) ++ ctxG) Gl' /\ (ishParts p Gl' -> False)).
+    {
+      clear Hc Hf He Hg Hh H5 H7.
+      clear H H0.
+      revert Ha Hb Hd. revert g1 p Gl ctxG ctxJ. clear s s0 s1 l xs.
+      apply shift_to; try easy.
+    }
+    destruct H1 as (Gl',(H1,(H2,Htm))).
+    exists (gtth_send s s0 (Some (s1, Gl') :: xs)). exists (ctxJ ++ ctxG).
+    - split.
+      constructor; try easy. apply SList_b; try easy.
+      constructor; try easy.
+      - right. exists s1. exists Gl'. exists g1. split. easy. split. easy.
+        apply typ_gtth_pad_l; try easy.
+      - revert H7. apply Forall2_mono; intros.
+        destruct H3. left. easy.
+        right. destruct H3 as (s2,(g2,(g3,(Hta,(Htb,Htc))))). subst.
+        exists s2. exists g2. exists g3. split. easy. split. easy.
+        apply typ_gtth_pad_r with (ctxG := ctxG); try easy.
+    - split.
+      intros. inversion H3. subst. easy. subst. easy. subst.
+      destruct n.
+      - simpl in H12. inversion H12. subst. apply Hb. easy.
+      - apply Hf. apply ha_sendr with (n := n) (s := s2) (g := g); try easy.
+    - split.
+      clear Htm H2 H1 H7 H5 Hh He Hf Hd Hb Ha H0 H. revert Hg Hc.
+      revert p ctxG. clear s s0 s1 g1 l Gl xs Gl'.
+      induction ctxJ; intros; try easy. inversion Hg. subst. clear Hg.
+      specialize(IHctxJ p ctxG H2 Hc). constructor; try easy.
+    - inversion Hh. subst.
+      apply used_con with (ctxGLis := Some (noneLis (Datatypes.length ctxJ) ++ ctxG) :: ctxGLis); try easy.
+      apply cmconss with (t := ctxJ); try easy.
+      clear H10 H8 Htm H2 H1 H7 H5  Hh Hg He Hf Hd Hc Hb Ha H0 H.
+      clear ctxGLis Gl' xs Gl p l g1 s1 s s0.
+      induction ctxJ; intros; try easy. simpl. constructor.
+      constructor; try easy. 
+      destruct a. right. right. left. exists g. easy.
+      left. easy.
+    - constructor; try easy. right. exists (noneLis (Datatypes.length ctxJ) ++ ctxG).
+      exists s1. exists Gl'. easy.
+Qed.
+
+
+
+Lemma balanced_to_tree : forall G p,
+    wfgC G ->
+    isgPartsC p G ->
+    exists G' ctxG, 
+       typ_gtth ctxG G' G /\ (ishParts p G' -> False) /\
+       List.Forall (fun u => u = None \/ (exists q lsg, u = Some (gtt_send p q lsg) \/ u = Some (gtt_send q p lsg) \/ u = Some (gtt_end))) ctxG /\ usedCtx ctxG G'.
+Proof.
+  intros.
+  specialize(parts_to_word p G H0); intros.
+  destruct H1 as (w,(r,Ha)). pose proof H as Htt.
+  unfold wfgC in H. destruct H as (Gl,(Hb,(Hc,(Hd,He)))). clear Hb Hc Hd. clear Gl H0.
+  pose proof He as Ht.
+  unfold balancedG in He.
+  specialize(He nil w p r).
+  simpl in He.
+  assert(exists gn, gttmap G nil None gn).
+  {
+    destruct G. exists gnode_end. constructor.
+    exists (gnode_pq s s0). constructor.
+  }
+  destruct H as (gn, H). specialize(He gn H).
+  assert(gttmap G w None (gnode_pq p r) \/ gttmap G w None (gnode_pq r p)).
+  {
+    destruct Ha. right. easy. left. easy.
+  }
+  specialize(He H0). clear H H0. destruct He as (k, H).
+  clear Ha.
+  revert H Ht Htt. revert G p. clear w r gn.
+  induction k; intros.
+  - specialize(H nil).
+    assert(exists gn, gttmap G nil None gn).
+    {
+      destruct G. exists gnode_end. constructor.
+      exists (gnode_pq s s0). constructor.
+    }
+    destruct H0 as (gn, H0). inversion H0; try easy. subst.
+    - assert(exists w2 w0 : seq.seq fin,
+        [] = w2 ++ w0 /\
+        (exists r : string,
+           gttmap gtt_end w2 None (gnode_pq p r) \/ gttmap gtt_end w2 None (gnode_pq r p))).
+      {
+        apply H. left. easy.
+      }
+      clear H. destruct H1 as (w2,(w0,(Ha,Hb))). destruct w2; try easy. simpl in Ha. subst.
+      destruct Hb as (r, Hb).
+      destruct Hb. inversion H. inversion H.
+    - assert(exists w2 w0 : seq.seq fin,
+      [] = w2 ++ w0 /\
+      (exists r : string, gttmap G w2 None (gnode_pq p r) \/ gttmap G w2 None (gnode_pq r p))).
+      apply H. right. split. easy. exists gn. easy.
+      destruct H2 as (w2,(w0,(Ha,Hb))). destruct w2; try easy. simpl in Ha. subst.
+      clear H.
+      destruct Hb as (r, Hb).
+      destruct Hb.
+      - inversion H. subst.
+        exists (gtth_hol 0). exists [Some (gtt_send p r xs)].
+        split.
+        - constructor; try easy.
+        - split. intros. inversion H1.
+        - split. constructor; try easy. right. exists r. exists xs. left. easy.
+        - assert(usedCtx (extendLis 0 (Some (gtt_send p r xs))) (gtth_hol 0)). constructor.
+          simpl in H1. easy.
+      - inversion H. subst.
+        exists (gtth_hol 0). exists [Some (gtt_send r p xs)].
+        split.
+        - constructor; try easy.
+        - split. intros. inversion H1.
+        - split. constructor; try easy. right. exists r. exists xs. right. left. easy.
+        - assert(usedCtx (extendLis 0 (Some (gtt_send r p xs))) (gtth_hol 0)). constructor.
+          simpl in H1. easy.
+  - destruct G.
+    - exists (gtth_hol 0). exists [Some gtt_end].
+      split. constructor. easy.
+      split. intros. inversion H0.
+      split. constructor; try easy. right. exists p. exists nil. right. right. easy.
+      assert(usedCtx (extendLis 0 (Some (gtt_end))) (gtth_hol 0)). constructor. simpl in H0. easy.
+    - specialize(balanced_cont Ht); intros.
+      - case_eq (eqb p s); intros.
+        assert (p = s). apply eqb_eq; try easy. subst.
+        exists (gtth_hol 0). exists [Some (gtt_send s s0 l)].
+        - split. constructor. easy.
+        - split. intros. inversion H2.
+        - split. constructor; try easy. right. exists s0. exists l. left. easy.
+        - assert(usedCtx (extendLis 0 (Some (gtt_send s s0 l))) (gtth_hol 0)). constructor. simpl in H2. easy.
+      - case_eq (eqb p s0); intros.
+        assert (p = s0). apply eqb_eq; try easy. subst.
+        exists (gtth_hol 0). exists [Some (gtt_send s s0 l)].
+        - split. constructor. easy.
+        - split. intros. inversion H3.
+        - split. constructor; try easy. right. exists s. exists l. right. left. easy.
+        - assert(usedCtx (extendLis 0 (Some (gtt_send s s0 l))) (gtth_hol 0)). constructor. simpl in H2. easy.
+      - assert (p <> s). apply eqb_neq; try easy. 
+        assert (p <> s0). apply eqb_neq; try easy.
+        clear H1 H2.
+      assert(Forall (fun u => u = None \/ (exists s g, u = Some(s, g) /\
+        (forall w' : seq.seq fin,
+       gttmap g w' None gnode_end \/
+       Datatypes.length w' = k /\ (exists tc : gnode, gttmap g w' None tc) ->
+       exists w2 w0 : seq.seq fin,
+         w' = w2 ++ w0 /\
+         (exists r : string, gttmap g w2 None (gnode_pq p r) \/ gttmap g w2 None (gnode_pq r p)))
+      )) l).
+      {
+        apply Forall_forall; intros.
+        destruct x.
+        - specialize(in_some_implies_onth p0 l H1); intros.
+          destruct H2 as (n, H2). destruct p0.
+          right. exists s1. exists g. split. easy.
+          intros.
+          specialize(H (n :: w')).
+          assert(exists w2 w0 : seq.seq fin,
+            (n :: w')%SEQ = w2 ++ w0 /\
+            (exists r : string,
+               gttmap (gtt_send s s0 l) w2 None (gnode_pq p r) \/
+               gttmap (gtt_send s s0 l) w2 None (gnode_pq r p))).
+          {
+            apply H; try easy.
+            destruct H5. left. apply gmap_con with (st := s1) (gk := g); try easy.
+            right. destruct H5. split. simpl. apply eq_S. easy.
+            destruct H6. exists x.
+            apply gmap_con with (st := s1) (gk := g); try easy.
+          }
+          destruct H6 as (w2,(w0,(Ha,Hb))).
+          destruct w2.
+          - simpl in *. subst.
+            destruct Hb as (r, Hb). destruct Hb. inversion H6. subst. easy.
+            inversion H6. subst. easy.
+          - inversion Ha. subst.
+            exists w2. exists w0. split. easy.
+            destruct Hb as (r, Hb). exists r.
+            destruct Hb.
+            - left. inversion H6. subst. specialize(eq_trans (esym H14) H2); intros.
+              inversion H7. subst. easy.
+            - right. inversion H6. subst. specialize(eq_trans (esym H14) H2); intros.
+              inversion H7. subst. easy.
+        - left. easy.
+      }
+      assert(Forall (fun u => u = None \/ (exists s g, u = Some(s, g) /\
+        exists (G' : gtth) (ctxG : seq.seq (option gtt)),
+        typ_gtth ctxG G' g /\
+        (ishParts p G' -> False) /\
+        Forall
+          (fun u : option gtt =>
+           u = None \/
+           (exists (q : string) (lsg : seq.seq (option (sort * gtt))),
+              u = Some (gtt_send p q lsg) \/ u = Some (gtt_send q p lsg) \/ u = Some gtt_end)) ctxG /\
+        usedCtx ctxG G'
+      )) l). 
+      {
+        clear H Ht.
+        assert(s <> s0).
+        {
+          specialize(wfgC_triv s s0 l Htt); intros. easy.
+        }
+        specialize(wfgC_after_step_all H Htt); intros. clear H Htt.
+        revert H0 IHk H1 H3 H4 H2. revert k s s0 p.
+        induction l; intros; try easy.
+        inversion H1. subst. clear H1. inversion H0. subst. clear H0. inversion H2. subst. clear H2.
+        specialize(IHl k s s0 p).
+        assert(Forall
+        (fun u : option (sort * gtt) =>
+         u = None \/
+         (exists (s : sort) (g : gtt),
+            u = Some (s, g) /\
+            (exists (G' : gtth) (ctxG : seq.seq (option gtt)),
+               typ_gtth ctxG G' g /\
+               (ishParts p G' -> False) /\
+               Forall
+                 (fun u0 : option gtt =>
+                  u0 = None \/
+                  (exists (q : string) (lsg : seq.seq (option (sort * gtt))),
+                     u0 = Some (gtt_send p q lsg) \/ u0 = Some (gtt_send q p lsg) \/ u0 = Some gtt_end))
+                 ctxG /\ usedCtx ctxG G'))) l).
+         apply IHl; try easy.
+         constructor; try easy. clear H H9 H8 H7 IHl.
+         destruct H5. left. easy.
+         destruct H as (s1,(g1,(Ha,Hb))). subst. 
+         destruct H1; try easy.
+         destruct H as (s2,(g2,(Hc,Hd))). inversion Hc. subst.
+         destruct H6; try easy. destruct H as (s3,(g3,(He,Hf))). inversion He. subst.
+         specialize(IHk g3 p). right. exists s3. exists g3. split. easy. apply IHk; try easy.
+      }
+    clear H1 H0 Ht H IHk.
+    assert(SList l).
+    {
+      specialize(wfgC_triv s s0 l Htt); intros. easy.
+    }
+    clear Htt.
+    revert H H2 H3 H4. clear k. revert s s0 p.
+    induction l; intros; try easy.
+    specialize(SList_f a l H); intros. clear H.
+    inversion H2. subst. clear H2.
+    destruct H0.
+    - specialize(IHl s s0 p).
+      assert(exists (G' : gtth) (ctxG : seq.seq (option gtt)),
+        typ_gtth ctxG G' (gtt_send s s0 l) /\
+        (ishParts p G' -> False) /\
+        Forall
+          (fun u : option gtt =>
+           u = None \/
+           (exists (q : string) (lsg : seq.seq (option (sort * gtt))),
+              u = Some (gtt_send p q lsg) \/ u = Some (gtt_send q p lsg) \/ u = Some gtt_end)) ctxG /\
+        usedCtx ctxG G').
+      {
+        apply IHl; try easy.
+      }
+      clear H6 H IHl.
+      destruct H5.
+      - subst.
+        destruct H0 as (Gl,(ctxG,(Ha,(Hb,(Hc,Hd))))).
+        inversion Ha.
+        - subst.
+          specialize(some_onth_implies_In n ctxG (gtt_send s s0 l) H); intros.
+          specialize(Forall_forall (fun u : option gtt =>
+        u = None \/
+        (exists (q : string) (lsg : seq.seq (option (sort * gtt))),
+           u = Some (gtt_send p q lsg) \/ u = Some (gtt_send q p lsg) \/ u = Some gtt_end)) ctxG); intros.
+          destruct H1. specialize(H1 Hc). clear H2 Hc.
+          specialize(H1 (Some (gtt_send s s0 l)) H0). destruct H1; try easy.
+          destruct H1 as (q1,(lsg,He)).
+          - destruct He. inversion H1. subst. easy.
+          - destruct H1. inversion H1. subst. easy.
+          - inversion H1. 
+        - subst.
+          exists (gtth_send s s0 (None :: xs)). exists ctxG.
+          - split. constructor; try easy.
+            constructor; try easy. left. easy.
+          - split. 
+            intros. apply Hb. inversion H. subst. easy. subst. easy. subst.
+            destruct n; try easy.
+            apply ha_sendr with (n := n) (s := s1) (g := g); try easy.
+          - split. easy.
+          - inversion Hd. subst. apply used_con with (ctxGLis := (None :: ctxGLis)); try easy.
+            constructor; try easy.
+            constructor; try easy. left. easy.
+      - destruct H as (s1,(g1,(Ha,Hb))). subst.
+        specialize(ctx_merge s s0 s1 g1 l p); intros. apply H; try easy.
+    destruct H as (H1,(a0,H2)). subst. clear H6 IHl.
+    destruct H5; try easy.
+    destruct H as (s1,(g1,(Ha,Hb))). inversion Ha. subst. clear Ha.
+    destruct Hb as (Gl,(ctxG,(Hc,(Hd,(He,Hf))))).
+    exists (gtth_send s s0 [Some (s1, Gl)]). exists ctxG.
+    - split. constructor; try easy. constructor; try easy.
+      right. exists s1. exists Gl. exists g1. easy.
+    - split. intros. apply Hd. inversion H. subst. easy. subst. easy. 
+      subst. destruct n; try easy.
+      - simpl in H8. inversion H8. subst. easy.
+      - simpl in H8. destruct n; try easy.
+    - split. easy.
+    - apply used_con with (ctxGLis := [Some ctxG]); try easy.
+      - constructor.
+      - constructor; try easy. right. exists ctxG. exists s1. exists Gl. easy.
+Qed.
+
